Add efficient Map implementation based on AVL tree

src/LCF.Map.fst
@@ -1,27 +1,270 @@
 module LCF.Map
 
-// TODO: more efficient associative datastructure
+(*** Datatypes and invariants ***)
 
-type cmp_on (a:Type0) =
-  a -> a -> bool
+type ordering =
+  | Lt
+  | Eq
+  | Gt
 
-type map (a:Type0) (cmp:cmp_on a) (b:Type) =
-  list (a & b)
+type cmp_on_ (a:Type0) =
+  a -> a -> ordering
+
+type map_ (a:Type0) (cmp:cmp_on_ a) (b:Type) =
+  | Nil: map_ a cmp b
+  | Node: bf:int{-1 <= bf && bf <= 1} -> left:map_ a cmp b -> (a&b) -> right:map_ a cmp b -> map_ a cmp b
+
+val cmp_on_axioms: #a:Type0 -> cmp_on_ a -> Type0
+let cmp_on_axioms #a cmp =
+  ( //Reflexivity
+    forall a. cmp a a == Eq
+  ) /\ ( //Anti-symetry
+    forall a b.
+    (cmp a b == Lt ==> cmp b a == Gt) /\
+    (cmp a b == Eq ==> cmp b a == Eq) /\
+    (cmp a b == Gt ==> cmp b a == Lt)
+  ) /\ ( //Transitivity
+    forall a b c.
+    (cmp a b == Lt /\ cmp b c == Lt ==> cmp a c == Lt) /\
+    (cmp a b == Lt /\ cmp b c == Eq ==> cmp a c == Lt) /\
+    (cmp a b == Eq /\ cmp b c == Lt ==> cmp a c == Lt) /\
+    (cmp a b == Eq /\ cmp b c == Eq ==> cmp a c == Eq) /\
+    (cmp a b == Eq /\ cmp b c == Gt ==> cmp a c == Gt) /\
+    (cmp a b == Gt /\ cmp b c == Eq ==> cmp a c == Gt) /\
+    (cmp a b == Gt /\ cmp b c == Gt ==> cmp a c == Gt)
+  )
+
+val max: int -> int -> int
+let max a b = if a < b then b else a
+
+val height: #a:Type0 -> #cmp:cmp_on_ a -> #b:Type -> map_ a cmp b -> GTot nat
+let rec height #a #cmp #b m =
+  match m with
+  | Nil -> 0
+  | Node _ l _ r -> (max (height l) (height r)) + 1
+
+val bf_invariant: #a:Type0 -> #cmp:cmp_on_ a -> #b:Type -> map_ a cmp b -> Type0
+let rec bf_invariant #a #cmp #b m =
+  match m with
+  | Nil -> True
+  | Node bf l _ r -> (bf == (height r) - (height l)) /\ bf_invariant l /\ bf_invariant r
+
+val in_map: #a:Type0 -> #cmp:cmp_on_ a -> #b:Type -> map_ a cmp b -> a -> Type0
+let rec in_map #a #cmp #b m x0 =
+  match m with
+  | Nil -> False
+  | Node _ l (x,y) r -> (in_map l x0) \/ (cmp x0 x == Eq) \/ (in_map r x0)
+
+val bst_invariant: #a:Type0 -> #cmp:cmp_on_ a -> #b:Type -> map_ a cmp b -> Type0
+let rec bst_invariant #a #cmp #b m =
+  match m with
+  | Nil -> True
+  | Node _ l (x,y) r ->
+    (forall xl. in_map l xl ==> cmp xl x == Lt) /\
+    (forall xr. in_map r xr ==> cmp x xr == Lt) /\
+    (bst_invariant l /\ bst_invariant r)
+
+type cmp_on (a:Type0) = cmp:cmp_on_ a{cmp_on_axioms cmp}
+type map (a:Type0) (cmp:cmp_on a) (b:Type) = m:map_ a cmp b{bf_invariant m /\ bst_invariant m}
+
+(*** Helper functions for `cmp_on` ***)
+
+val cmp_on_lex: #a:Type0 -> #b:Type0 -> cmp_on a -> cmp_on b -> cmp_on (a&b)
+let cmp_on_lex #a #b cmpa cmpb (xa,xb) (ya,yb) =
+  match cmpa xa ya with
+  | Lt -> Lt
+  | Gt -> Gt
+  | Eq -> cmpb xb yb
+
+val cmp_on_option: #a:Type0 -> cmp_on a -> cmp_on (option a)
+let cmp_on_option #a cmp ox oy =
+  match ox, oy with
+  | None, None -> Eq
+  | Some x, None -> Gt
+  | None, Some y -> Lt
+  | Some x, Some y -> cmp x y
+
+val cmp_on_list_leq_n: #n:nat -> #a:Type0 -> cmp_on a -> cmp_on (l:list a{List.Tot.length l <= n})
+let rec cmp_on_list_leq_n #n #a cmp (lx:(l:list a{List.Tot.length l <= n})) (ly:(l:list a{List.Tot.length l <= n})) =
+  match lx, ly with
+  | [], [] -> Eq
+  | x::xs, [] -> Gt
+  | [], y::ys -> Lt
+  | x::xs, y::ys ->
+    begin
+      cmp_on_lex cmp (cmp_on_list_leq_n #(n-1) cmp) (x,xs) (y,ys)
+    end
+
+val cmp_on_list_: #a:Type0 -> cmp_on a -> list a -> list a -> ordering
+let rec cmp_on_list_ #a cmp lx ly =
+  match lx, ly with
+  | [], [] -> Eq
+  | x::xs, [] -> Gt
+  | [], y::ys -> Lt
+  | x::xs, y::ys ->
+    begin
+      match cmp x y with
+      | Lt -> Lt
+      | Gt -> Gt
+      | Eq -> cmp_on_list_ cmp xs ys
+    end
+
+//If you find a prettier way to define this function, I would happily buy you a beer!
+val cmp_on_list: #a:Type0 -> cmp_on a -> cmp_on (list a)
+let cmp_on_list #a cmp =
+  let rec cmp_on_list_eq_cmp_on_list_leq_n (#a:Type0) (cmp:cmp_on a) (n:nat) (lx:list a) (ly:list a): Lemma
+    ((List.Tot.length lx <= n /\ List.Tot.length ly <= n) ==> cmp_on_list_ cmp lx ly == cmp_on_list_leq_n #n cmp lx ly) =
+    match lx,ly with
+    | x::xs, y::ys -> if (n <= 0) then () else cmp_on_list_eq_cmp_on_list_leq_n cmp (n-1) xs ys
+    | _ -> ()
+  in
+  FStar.Classical.forall_intro_3 (cmp_on_list_eq_cmp_on_list_leq_n #a cmp);
+  assert (forall (lx:list a) (ly:list a).
+    let n = max (List.Tot.length lx) (List.Tot.length ly) in
+    cmp_on_list_ cmp lx ly == cmp_on_list_leq_n #n cmp lx ly
+  );
+  //The following assert can be removed, but I don't understand how?
+  assert (forall (lx:list a) (ly:list a) (lz:list a).
+    let n = max (max (List.Tot.length lx) (List.Tot.length ly)) (List.Tot.length lz) in
+    cmp_on_list_ cmp lx ly == cmp_on_list_leq_n #n cmp lx ly /\
+    cmp_on_list_ cmp lx lz == cmp_on_list_leq_n #n cmp lx lz /\
+    cmp_on_list_ cmp ly lz == cmp_on_list_leq_n #n cmp ly lz
+  );
+  cmp_on_list_ cmp
+
+(*** Map definition ***)
 
 val map_empty: #a:Type0 -> #cmp:cmp_on a -> #b:Type -> map a cmp b
 let map_empty #a #cmp #b =
-  []
+  Nil
 
 val map_is_empty: #a:Type0 -> #cmp:cmp_on a -> #b:Type -> map a cmp b -> bool
 let map_is_empty #a #cmp #b m =
   match m with
-  | [] -> true
+  | Nil -> true
   | _ -> false
 
-val map_lookup: #a:Type0 -> #cmp:cmp_on a -> #b:Type -> map a cmp b -> a -> option b
-let map_lookup #a #cmp #b m x0 =
-    List.Tot.fold_right (fun (x, y) acc -> if cmp x x0 then Some y else acc) m None
+val map_lookup: #a:Type0 -> #cmp:cmp_on a -> #b:Type -> m:map a cmp b -> x0:a -> Pure (option b)
+  (requires True)
+  (ensures fun res -> (Some? res) <==> in_map m x0)
+let rec map_lookup #a #cmp #b m x0 =
+  match m with
+  | Nil -> None
+  | Node bf l (x,y) r ->
+    begin
+      match cmp x0 x with
+      | Lt -> map_lookup l x0
+      | Eq -> Some y
+      | Gt -> map_lookup r x0
+    end
 
-val map_insert: #a:Type0 -> #cmp:cmp_on a -> #b:Type -> map a cmp b -> a -> b -> map a cmp b
-let map_insert #a #b m x y =
-  (x,y)::m
+#push-options "--z3rlimit 30"
+val rotate_right: #a:Type0 -> #cmp:cmp_on a -> #b:Type -> l:map a cmp b -> x:(a&b) -> r:map a cmp b -> Pure (map a cmp b & bool)
+  (requires
+    (height r) - (height l) == -2 /\
+    (forall xl. in_map l xl ==> cmp xl (fst x) == Lt) /\ (forall xr. in_map r xr ==> cmp (fst x) xr == Lt)
+  )
+  (ensures fun (res, height_unchanged) ->
+    height res == (max (height l) (height r)) + 1 + (if height_unchanged then 0 else -1) /\
+    (forall x0. in_map res x0 <==> (in_map l x0) \/ (cmp x0 (fst x) == Eq) \/ (in_map r x0))
+  )
+let rotate_right #a #cmp #b l x r =
+  match l with
+  | Node lbf ll lx lr ->
+    begin
+      if lbf = -1 then
+        (Node 0 ll lx (Node 0 lr x r) , false)
+      else if lbf = 0 then
+        (Node 1 ll lx (Node (-1) lr x r), true)
+      else (
+        match lr with
+        | Node lrbf lrl lrx lrr ->
+          begin
+            let b1 = if lrbf = 1 then -1 else 0 in
+            let b2 = if lrbf = -1 then 1 else 0 in
+            (Node 0 (Node b1 ll lx lrl) lrx (Node b2 lrr x r), false)
+          end
+      )
+    end
+#pop-options
+
+#push-options "--z3rlimit 30"
+val rotate_left: #a:Type0 -> #cmp:cmp_on a -> #b:Type -> l:map a cmp b -> x:(a&b) -> r:map a cmp b -> Pure (map a cmp b & bool)
+  (requires
+    (height r) - (height l) == 2 /\
+    (forall xl. in_map l xl ==> cmp xl (fst x) == Lt) /\ (forall xr. in_map r xr ==> cmp (fst x) xr == Lt)
+  )
+  (ensures fun (res, height_unchanged) ->
+    height res == (max (height l) (height r)) + 1 + (if height_unchanged then 0 else -1) /\
+    (forall x0. in_map res x0 <==> (in_map l x0) \/ (cmp x0 (fst x) == Eq) \/ (in_map r x0))
+  )
+let rotate_left #a #cmp #b l x r =
+  match r with
+  | Node rbf rl rx rr ->
+    begin
+      if rbf = 1 then
+        (Node 0 (Node 0 l x rl) rx rr, false)
+      else if rbf = 0 then
+        (Node (-1) (Node 1 l x rl) rx rr, true)
+      else
+        match rl with
+        | Node rlbf rll rlx rlr ->
+          begin
+            let b1 = if rlbf = 1 then -1 else 0 in
+            let b2 = if rlbf = -1 then 1 else 0 in
+            (Node 0 (Node b1 l x rll) rlx (Node b2 rlr rx rr), false)
+          end
+    end
+#pop-options
+
+#push-options "--z3rlimit 30"
+val map_insert_aux: #a:Type0 -> #cmp:cmp_on a -> #b:Type -> m:map a cmp b -> x0:a -> b -> Pure (map a cmp b & bool)
+  (requires True)
+  (ensures fun (res, height_increased) ->
+    height res = (height m) + (if height_increased then 1 else 0) /\
+    (forall x. in_map res x <==> (in_map m x \/ cmp x0 x == Eq))
+  )
+let rec map_insert_aux #a #cmp #b m x0 y0 =
+  match m with
+  | Nil -> (Node 0 Nil (x0, y0) Nil, true)
+  | Node bf l (x,y) r ->
+    begin
+      match cmp x0 x with
+      | Lt ->
+        begin
+          let (l_new, height_increased) = map_insert_aux l x0 y0 in
+          if height_increased then (
+            if bf = -1 then (
+              rotate_right l_new (x,y) r
+            )
+            else if bf = 0 then
+              (Node (-1) l_new (x,y) r, true)
+            else
+              (Node 0 l_new (x,y) r, false)
+          ) else (
+            (Node bf l_new (x,y) r, false)
+          )
+        end
+      | Eq -> (Node bf l (x0,y0) r, false)
+      | Gt ->
+        begin
+          let (r_new, height_increased) = map_insert_aux r x0 y0 in
+          if height_increased then (
+            if bf = -1 then
+              (Node 0 l (x,y) r_new, false)
+            else if bf = 0 then
+              (Node 1 l (x,y) r_new, true)
+            else
+              rotate_left l (x,y) r_new
+          ) else (
+            (Node bf l (x,y) r_new, false)
+          )
+        end
+    end
+#pop-options
+
+val map_insert: #a:Type0 -> #cmp:cmp_on a -> #b:Type -> m:map a cmp b -> x0:a -> b -> Pure (map a cmp b)
+  (requires True)
+  (ensures fun res -> forall x. in_map res x <==> (in_map m x \/ cmp x0 x == Eq))
+let map_insert #a #cmp #b m x0 y0 =
+  fst (map_insert_aux m x0 y0)
